Pull out bits of RGA_Spec into abstract OpSet theory

isabelle/RGA_Spec.thy
@@ -1,342 +1,52 @@
 theory RGA_Spec
-  imports Main Permute Insert_Spec RGA
+  imports OpSet Insert_Spec RGA
 begin
 
-inductive valid_spec_ops :: "('oid::{linorder} \<times> 'oid option) list \<Rightarrow> bool" where
-  "valid_spec_ops []" |
-  "\<lbrakk>valid_spec_ops xs;
-    \<forall>x \<in> set (map fst xs). x < oid\<rbrakk> \<Longrightarrow> valid_spec_ops (xs@[(oid, None)])" |
-  "\<lbrakk>valid_spec_ops xs;
-    \<forall>x \<in> set (map fst xs). x < oid; ref < oid\<rbrakk> \<Longrightarrow> valid_spec_ops (xs@[(oid, Some ref)])"
-
-inductive valid_rga_ops :: "('oid::{linorder} \<times> 'oid option) list \<Rightarrow> bool" where
-  "valid_rga_ops []" |
-  "\<lbrakk>valid_rga_ops xs;
-    oid \<notin> set (map fst xs)\<rbrakk> \<Longrightarrow> valid_rga_ops (xs@[(oid, None)])" |
-  "\<lbrakk>valid_rga_ops xs;
-    oid \<notin> set (map fst xs);
-    ref \<in> set (map fst xs); ref < oid\<rbrakk>  \<Longrightarrow> valid_rga_ops (xs@[(oid, Some ref)])"
-
-subsection\<open>Lemmata about the valid_spec_ops predicate\<close>
-
-inductive_cases spec_ops_last: "valid_spec_ops (xs @ [x])"
-
-lemma spec_ops_distinct:
-  assumes "valid_spec_ops xs"
-  shows "distinct xs"
-  using assms by(induction rule: valid_spec_ops.induct, force+)
-
-lemma spec_ops_sorted:
-  assumes "valid_spec_ops xs"
-  shows "sorted (map fst xs)"
-  using assms by (induction rule: valid_spec_ops.induct; auto simp add: order_less_imp_le sorted_append)
-
-lemma spec_ops_ref_less:
-  assumes "valid_spec_ops (xs @ [(oid, Some ref)])"
-  shows "ref < oid"
-  using assms valid_spec_ops.cases by force
-
-lemma spec_ops_rem_last:
-  assumes "valid_spec_ops (xs@[x])"
-  shows "valid_spec_ops xs"
-  using assms valid_spec_ops.cases by fastforce
-
-lemma spec_ops_id_inc:
-  assumes "valid_spec_ops (xs@[(oid,ref)])"
-    and "x \<in> set (map fst xs)"
-  shows "x < oid"
-  using assms valid_spec_ops.cases snoc_eq_iff_butlast by auto
-
-lemma spec_ops_add_any:
-  assumes "valid_spec_ops (xs @ ys)"
-    and "\<forall>i \<in> set (map fst xs). i < oid"
-    and "\<forall>i \<in> set (map fst ys). oid < i"
-    and "\<And>r. ref = Some r \<Longrightarrow> r < oid"
-  shows "valid_spec_ops (xs @ [(oid, ref)] @ ys)"
-using assms proof(induction ys rule: rev_induct)
-  case Nil
-  then show "valid_spec_ops (xs @ [(oid, ref)] @ [])"
-    by (cases ref, auto simp add: valid_spec_ops.intros)
-next
-  case (snoc y ys)
-  have IH: "valid_spec_ops (xs @ [(oid, ref)] @ ys)"
-  proof -
-    from snoc have "valid_spec_ops (xs @ ys)"
-      by (metis append_assoc spec_ops_rem_last)
-    thus "valid_spec_ops (xs @ [(oid, ref)] @ ys)"
-      using assms(2) snoc by auto
-  qed
-  obtain yi yr where y_pair: "y = (yi, yr)"
-    by force
-  have oid_yi: "oid < yi"
-    by (simp add: snoc.prems(3) y_pair)
-  have yi_biggest: "\<forall>i \<in> set (map fst (xs @ (oid, ref) # ys)). i < yi"
-  proof -
-    have "\<forall>i \<in> set (map fst xs). i < yi"
-      using oid_yi assms(2) less_trans by blast
-    moreover have "\<forall>i \<in> set (map fst ys). i < yi"
-      by (metis UnCI append_assoc map_append set_append snoc.prems(1) spec_ops_id_inc y_pair)
-    ultimately show ?thesis
-      using oid_yi by auto
-  qed
-  thus "valid_spec_ops (xs @ [(oid, ref)] @ ys @ [y])"
-  proof(cases yr)
-    case None
-    then show ?thesis
-      using IH yi_biggest valid_spec_ops.intros(2) y_pair by fastforce
-  next
-    case (Some r)
-    moreover have "r < yi"
-      by (metis Some append_assoc snoc.prems(1) spec_ops_ref_less y_pair)
-    ultimately show ?thesis
-      using IH yi_biggest valid_spec_ops.intros(3) y_pair by fastforce
-  qed
-qed
-
-lemma spec_ops_split:
-  assumes "valid_spec_ops xs"
-    and "oid \<notin> set (map fst xs)"
-  shows "\<exists>pre suf. xs = pre @ suf \<and>
-            (\<forall>i \<in> set (map fst pre). i < oid) \<and>
-            (\<forall>i \<in> set (map fst suf). oid < i)"
-using assms proof(induction xs rule: rev_induct)
-  case Nil
-  then show ?case by force
-next
-  case (snoc x xs)
-  obtain xi xr where y_pair: "x = (xi, xr)"
-    by force
-  obtain pre suf where IH: "xs = pre @ suf \<and>
-               (\<forall>a\<in>set (map fst pre). a < oid) \<and>
-               (\<forall>a\<in>set (map fst suf). oid < a)"
-    by (metis UnCI map_append set_append snoc spec_ops_rem_last)
-  then show ?case
-  proof(cases "xi < oid")
-    case xi_less: True
-    have "\<forall>x \<in> set (map fst (pre @ suf)). x < xi"
-      using IH spec_ops_id_inc snoc.prems(1) y_pair by blast
-    hence "\<forall>x \<in> set suf. fst x < xi"
-      by simp
-    hence "\<forall>x \<in> set suf. fst x < oid"
-      using xi_less by auto
-    hence "suf = []"
-      using IH last_in_set by fastforce
-    hence "xs @ [x] = (pre @ [(xi, xr)]) @ [] \<and>
-              (\<forall>a\<in>set (map fst ((pre @ [(xi, xr)]))). a < oid) \<and>
-              (\<forall>a\<in>set (map fst []). oid < a)"
-      by (simp add: IH xi_less y_pair)
-    then show ?thesis by force
-  next
-    case False
-    hence "oid < xi" using snoc.prems(2) y_pair by auto
-    hence "xs @ [x] = pre @ (suf @ [(xi, xr)]) \<and>
-              (\<forall>i \<in> set (map fst pre). i < oid) \<and>
-              (\<forall>i \<in> set (map fst (suf @ [(xi, xr)])). oid < i)"
-      by (simp add: IH y_pair)
-    then show ?thesis by blast
-  qed
-qed
+locale insert_opset = opset opset set_option
+  for opset :: "('oid::{linorder} \<times> 'oid option) set"
 
 
-subsection\<open>Lemmata about the valid_rga_ops predicate\<close>
+subsection\<open>Lemmata about the rga_ops predicate\<close>
 
-lemma rga_ops_intro:
-  assumes "\<And>r. ref = Some r \<Longrightarrow> r \<in> fst ` set xs \<and> r < oid"
-    and "oid \<notin> fst ` set xs"
-    and "valid_rga_ops xs"
-  shows "valid_rga_ops (xs @ [(oid, ref)])"
-using assms by (cases ref; auto simp add: valid_rga_ops.intros)
+definition rga_ops :: "('oid::{linorder} \<times> 'oid option) list \<Rightarrow> bool" where
+  "rga_ops list \<equiv> crdt_ops set_option list \<and> insert_opset (set list)"
 
 lemma rga_ops_rem_last:
-  assumes "valid_rga_ops (xs@[x])"
-  shows "valid_rga_ops xs"
-using assms valid_rga_ops.cases by fastforce
+  assumes "rga_ops (xs @ [x])"
+  shows "rga_ops xs"
+using assms proof -
+  have "crdt_ops set_option xs"
+    using assms crdt_ops_rem_last rga_ops_def by blast
+  moreover have "insert_opset (set xs)"
+    using assms opset_insert insert_opset.axioms insert_opset.intro
+    by (metis list.simps(15) rga_ops_def rotate1.simps(2) set_rotate1)
+  ultimately show "rga_ops xs"
+    by (simp add: rga_ops_def)
+qed
 
-lemma rga_ops_ref_less_mid:
-  assumes "valid_rga_ops xs"
-    and "(oid, Some ref) \<in> set xs"
-  shows "ref < oid"
-using assms by (induction rule: valid_rga_ops.induct, auto)
-
-lemma rga_ops_ref_less_last:
-  assumes "valid_rga_ops (xs @ [(oid, Some ref)])"
-  shows "ref < oid"
-using assms rga_ops_ref_less_mid by fastforce
-
-lemma rga_ops_distinct:
-  assumes "valid_rga_ops xs"
-  shows "distinct xs"
-using assms by (induction xs, force+)
-
-lemma rga_ops_distinct_fst:
-  assumes "valid_rga_ops xs"
-  shows "distinct (map fst xs)"
-using assms by (induction xs, auto)
-
-lemma rga_ops_unique_last:
-  assumes "valid_rga_ops (xs @ [(oid, ref)])"
-  shows "oid \<notin> set (map fst xs)"
-using assms valid_rga_ops.cases by blast
-
-lemma rga_ops_unique_mid:
-  assumes "valid_rga_ops (xs @ [(oid, ref)] @ ys)"
-  shows "oid \<notin> set (map fst xs) \<and> oid \<notin> set (map fst ys)"
-using assms proof(induction ys rule: rev_induct)  
-  case Nil
-  then show "oid \<notin> set (map fst xs) \<and> oid \<notin> set (map fst [])"
-    using valid_rga_ops.cases snoc_eq_iff_butlast by auto
-next
-  case (snoc y ys)
-  obtain yi yr where y_pair: "y = (yi, yr)"
-    by fastforce
-  have IH: "oid \<notin> set (map fst xs) \<and> oid \<notin> set (map fst ys)"
-    using rga_ops_rem_last snoc by (metis append_assoc)
-  have "(xs @ (oid, ref) # ys) @ [(yi, yr)] = xs @ (oid, ref) # ys @ [(yi, yr)]"
-    by simp
-  hence "yi \<notin> set (map fst (xs @ (oid, ref) # ys))"
-    using rga_ops_unique_last by (metis append_Cons append_self_conv2 snoc.prems y_pair)
-  thus "oid \<notin> set (map fst xs) \<and> oid \<notin> set (map fst (ys @ [y]))"
-    using IH y_pair by auto
+lemma rga_ops_rem_penultimate:
+  assumes "rga_ops (xs @ [(i1, r1), (i2, r2)])"
+    and "\<And>r. r2 = Some r \<Longrightarrow> r \<noteq> i1"
+  shows "rga_ops (xs @ [(i2, r2)])"
+using assms proof -
+  have "crdt_ops set_option (xs @ [(i2, r2)])"
+    using assms crdt_ops_rem_penultimate rga_ops_def by fastforce
+  moreover have "insert_opset (set (xs @ [(i2, r2)]))"
+    using assms(1) insert_opset.axioms insert_opset.intro opset_insert rga_ops_def by force
+  ultimately show "rga_ops (xs @ [(i2, r2)])"
+    by (simp add: rga_ops_def)
 qed
 
 lemma rga_ops_ref_exists:
-  assumes "valid_rga_ops (pre @ (oid, Some ref) # suf)"
+  assumes "rga_ops (pre @ (oid, Some ref) # suf)"
   shows "ref \<in> fst ` set pre"
-using assms proof(induction suf rule: List.rev_induct)
-  case Nil thus ?case using valid_rga_ops.cases by fastforce
-next
-  case (snoc x xs) thus ?case using valid_rga_ops.cases by fastforce
-qed
-
-lemma rga_ops_no_future_ref:
-  assumes "valid_rga_ops (xs @ [(oid, ref)] @ ys)"
-  shows "\<And>r. ref = Some r \<Longrightarrow> r \<notin> fst ` set ys"
 proof -
-  from assms(1) have "\<And>r. ref = Some r \<Longrightarrow> r \<in> set (map fst xs)"
-    by (simp add: rga_ops_ref_exists)
-  moreover have "distinct (map fst (xs @ [(oid, ref)] @ ys))"
-    using assms rga_ops_distinct_fst by blast
-  ultimately have "\<And>r. ref = Some r \<Longrightarrow> r \<notin> set (map fst ([(oid, ref)] @ ys))"
-    using distinct_pair_list_memb by metis
-  thus "\<And>r. ref = Some r \<Longrightarrow> r \<notin> fst ` set ys"
+  from assms have "crdt_ops set_option (pre @ (oid, Some ref) # suf)"
+    by (simp add: rga_ops_def)
+  moreover have "set_option (Some ref) = {ref}"
     by simp
-qed
-
-lemma rga_ops_reorder:
-  assumes "valid_rga_ops (xs @ [(oid, ref)] @ ys)"
-    and "\<And>r. Some r \<in> snd ` set ys \<Longrightarrow> r \<noteq> oid"
-  shows "valid_rga_ops (xs @ ys @ [(oid, ref)])"
-using assms proof(induction ys rule: rev_induct)
-  case Nil
-  then show "valid_rga_ops (xs @ [] @ [(oid, ref)])"
-    using rga_ops_rem_last by auto
-next
-  case (snoc y ys)
-  then obtain yi yr where y_pair: "y = (yi, yr)"
-    by force
-  have IH: "valid_rga_ops (xs @ ys @ [(oid, ref)])"
-  proof -
-    have "valid_rga_ops (xs @ [(oid, ref)] @ ys)"
-      by (metis snoc(2) append.assoc rga_ops_rem_last)
-    thus "valid_rga_ops (xs @ ys @ [(oid, ref)])"
-      using snoc.IH snoc.prems(2) by auto
-  qed
-  have "valid_rga_ops (xs @ ys @ [y])"
-  proof -
-    have "yi \<notin> fst ` set (xs @ [(oid, ref)] @ ys)"
-      by (metis y_pair append_assoc rga_ops_unique_last set_map snoc.prems(1))
-    hence "yi \<notin> fst ` set (xs @ ys)"
-      by auto
-    moreover have "\<And>r. yr = Some r \<Longrightarrow> r \<in> fst ` set (xs @ ys)"
-    proof -
-      have "\<And>r. yr = Some r \<Longrightarrow> r \<noteq> oid"
-        by (simp add: y_pair snoc.prems(2))
-      moreover have "\<And>r. yr = Some r \<Longrightarrow> r \<in> fst ` set (xs @ [(oid, ref)] @ ys)"
-        by (metis y_pair append_assoc snoc.prems(1) rga_ops_ref_exists)
-      ultimately show "\<And>r. yr = Some r \<Longrightarrow> r \<in> fst ` set (xs @ ys)"
-        by simp
-    qed
-    moreover have "\<And>r. yr = Some r \<Longrightarrow> r < yi"
-      using snoc.prems(1) rga_ops_ref_less_mid y_pair by fastforce
-    moreover from IH have "valid_rga_ops (xs @ ys)"
-      using rga_ops_rem_last by force
-    ultimately show "valid_rga_ops (xs @ ys @ [y])"
-      using y_pair rga_ops_intro by (metis append_assoc)
-  qed
-  moreover have "oid \<notin> fst ` set (xs @ ys @ [y])"
-    using rga_ops_unique_mid by (metis (no_types, lifting) UnE image_Un 
-      image_set set_append snoc.prems(1))
-  moreover have "\<And>r. ref = Some r \<Longrightarrow> r \<in> fst ` set (xs @ ys @ [y])"
-    using rga_ops_ref_exists
-    by (metis UnCI append_Cons image_Un set_append snoc.prems(1))
-  moreover have "\<And>r. ref = Some r \<Longrightarrow> r < oid"
-    using IH by (simp add: rga_ops_ref_less_mid)
-  ultimately show "valid_rga_ops (xs @ (ys @ [y]) @ [(oid, ref)])"
-    using rga_ops_intro by (metis append_assoc)
-qed
-
-lemma rga_ops_rem_middle:
-  assumes "valid_rga_ops (xs @ [(oid, ref)] @ ys)"
-    and "\<And>r. Some r \<in> snd ` set ys \<Longrightarrow> r \<noteq> oid"
-  shows "valid_rga_ops (xs @ ys)"
-using assms rga_ops_rem_last rga_ops_reorder append_assoc by metis
-
-lemma rga_ops_independent_suf:
-  assumes "valid_spec_ops (xs @ [(oid, ref)])"
-    and "valid_rga_ops (ys @ [(oid, ref)] @ zs)"
-    and "permut (xs @ [(oid, ref)]) (ys @ [(oid, ref)] @ zs)"
-  shows "\<And>i r. (i, Some r) \<in> set zs \<Longrightarrow> r \<noteq> oid"
-proof -
-  have "\<And>i r. (i, Some r) \<in> set xs \<Longrightarrow> r < oid"
-  proof -
-    from assms(1) have "\<And>i. i \<in> fst ` set xs \<Longrightarrow> i < oid"
-      using spec_ops_id_inc by fastforce
-    moreover from assms(1) have "\<And>i r. (i, Some r) \<in> set xs \<Longrightarrow> r < i"
-      using assms rga_ops_ref_less_mid by (metis butlast_snoc in_set_butlastD permut_def)
-    ultimately show "\<And>i r. (i, Some r) \<in> set xs \<Longrightarrow> r < oid"
-      by fastforce
-  qed
-  moreover from assms(3) have "set zs \<subseteq> set xs"
-    by (metis permut_rem_last permut_subset(2))
-  ultimately show "\<And>i r. (i, Some r) \<in> set zs \<Longrightarrow> r \<noteq> oid"
-    by fastforce
-qed
-
-lemma rga_ops_reorder_spec:
-  assumes "valid_spec_ops (xs @ [(oid, ref)])"
-    and "valid_rga_ops (ys @ [(oid, ref)] @ zs)"
-    and "permut (xs @ [(oid, ref)]) (ys @ [(oid, ref)] @ zs)"
-  shows "valid_rga_ops (ys @ zs @ [(oid, ref)])"
-using assms rga_ops_reorder rga_ops_independent_suf by fastforce
-
-lemma rga_ops_rem_spec:
-  assumes "valid_spec_ops (xs @ [(oid, ref)])"
-    and "valid_rga_ops (ys @ [(oid, ref)] @ zs)"
-    and "permut (xs @ [(oid, ref)]) (ys @ [(oid, ref)] @ zs)"
-  shows "valid_rga_ops (ys @ zs)"
-using assms rga_ops_rem_last rga_ops_reorder_spec append_assoc by metis
-
-lemma rga_ops_rem_penultimate:
-  assumes "valid_rga_ops (xs @ [(i1, r1)] @ [(i2, r2)])"
-    and "\<And>r. r2 = Some r \<Longrightarrow> r \<noteq> i1"
-  shows "valid_rga_ops (xs @ [(i2, r2)])"
-proof -
-  have "valid_rga_ops (xs @ [(i1, r1)])"
-    using assms(1) rga_ops_rem_last by force
-  hence "valid_rga_ops xs"
-    using rga_ops_rem_last by force
-  moreover have "distinct (map fst (xs @ [(i1, r1)] @ [(i2, r2)]))"
-    using assms(1) rga_ops_distinct_fst by blast
-  hence "i2 \<notin> set (map fst xs)"
-    by auto
-  moreover have "\<And>r. r2 = Some r \<Longrightarrow> r \<in> set (map fst (xs @ [(i1, r1)]))"
-    using assms(1) by (metis append.assoc list.set_map rga_ops_ref_exists)
-  hence "\<And>r. r2 = Some r \<Longrightarrow> r \<in> set (map fst xs)"
-    using assms(2) by auto
-  moreover have "\<And>r. r2 = Some r \<Longrightarrow> r < i2"
-    using assms(1) rga_ops_ref_less_last by (metis append.assoc)
-  ultimately show "valid_rga_ops (xs @ [(i2, r2)])"
-    by (simp add: rga_ops_intro)
+  ultimately show "ref \<in> fst ` set pre"
+    using crdt_ops_ref_exists by fastforce
 qed
 
 
@@ -347,7 +57,7 @@ lemma interp_rga_tail_unfold:
 by (clarsimp simp add: interp_rga_def)
 
 lemma interp_rga_ids:
-  assumes "valid_rga_ops xs"
+  assumes "rga_ops xs"
   shows "set (interp_rga xs) = set (map fst xs)"
 using assms proof(induction xs rule: List.rev_induct)
   case Nil
@@ -357,8 +67,7 @@ next
   case (snoc x xs)
   hence IH: "set (interp_rga xs) = set (map fst xs)"
     using rga_ops_rem_last by blast
-  obtain xi xr where x_pair: "x = (xi, xr)"
-    by force
+  obtain xi xr where x_pair: "x = (xi, xr)" by force
   then show "set (interp_rga (xs @ [x])) = set (map fst (xs @ [x]))"
   proof(cases xr)
     case None
@@ -376,7 +85,7 @@ next
 qed
 
 lemma interp_rga_distinct:
-  assumes "valid_rga_ops xs"
+  assumes "rga_ops xs"
   shows "distinct (interp_rga xs)"
 using assms proof(induction xs rule: List.rev_induct)
   case Nil
@@ -388,14 +97,20 @@ next
   moreover obtain xi xr where x_pair: "x = (xi, xr)"
     by force
   moreover from this have "xi \<notin> set (interp_rga xs)"
-    using interp_rga_ids rga_ops_unique_last rga_ops_rem_last by (metis snoc.prems)
-  moreover have "xr = None \<or> (\<exists>r. xr = Some r \<and> r \<in> set (map fst xs))"
-    using valid_rga_ops.cases snoc.prems snoc_eq_iff_butlast x_pair by auto
-  hence "xr = None \<or> (\<exists>r. xr = Some r \<and> r \<in> set (interp_rga xs))"
-    using interp_rga_ids rga_ops_rem_last snoc.prems by blast
-  hence "\<exists>pre suf. interp_rga xs = pre@suf \<and>
+    using interp_rga_ids crdt_ops_unique_last rga_ops_rem_last
+    by (metis rga_ops_def snoc.prems)
+  moreover have "\<exists>pre suf. interp_rga xs = pre@suf \<and>
            insert_rga (interp_rga xs) (xi, xr) = pre @ xi # suf"
-    using IH insert_preserves_order by blast
+  proof -
+    have "\<And>r. r \<in> set_option xr \<Longrightarrow> r \<in> set (map fst xs)"
+      using crdt_ops_ref_exists rga_ops_def snoc.prems x_pair by fastforce
+    hence "xr = None \<or> (\<exists>r. xr = Some r \<and> r \<in> set (map fst xs))"
+      using option.set_sel by blast
+    hence "xr = None \<or> (\<exists>r. xr = Some r \<and> r \<in> set (interp_rga xs))"
+      using interp_rga_ids rga_ops_rem_last snoc.prems by blast
+    thus ?thesis
+      using IH insert_preserves_order by blast
+  qed
   ultimately show "distinct (interp_rga (xs @ [x]))" 
     by (metis Un_iff disjoint_insert(1) distinct.simps(2) distinct_append 
         interp_rga_tail_unfold list.simps(15) set_append)
@@ -406,8 +121,8 @@ subsection\<open>Proof that RGA satisfies the list specification\<close>
 
 lemma final_insert:
   assumes "permut (xs @ [x]) (ys @ [x])"
-    and "valid_rga_ops (xs @ [x])"
-    and "valid_spec_ops (ys @ [x])"
+    and "rga_ops (xs @ [x])"
+    and "spec_ops (ys @ [x])"
     and "interp_rga xs = interp_list ys"
   shows "interp_rga (xs @ [x]) = interp_list (ys @ [x])"
 proof -
@@ -417,7 +132,7 @@ proof -
   have oid_greatest: "\<And>i. i \<in> set (interp_rga xs) \<Longrightarrow> i < oid"
   proof -
     have "\<And>i. i \<in> set (map fst ys) \<Longrightarrow> i < oid"
-      using assms(3) spec_ops_id_inc x_pair by blast
+      using assms(3) by (simp add: spec_ops_id_inc x_pair)
     hence "\<And>i. i \<in> set (map fst xs) \<Longrightarrow> i < oid"
       using \<open>permut xs ys\<close> permut_pair_fst by blast
     thus "\<And>i. i \<in> set (interp_rga xs) \<Longrightarrow> i < oid"
@@ -436,7 +151,7 @@ proof -
     have "\<exists>as bs. interp_rga xs = as @ r # bs"
     proof -
       have "r \<in> set (map fst xs)"
-        using assms(2) valid_rga_ops.cases Some x_pair by blast
+        using assms(2) Some by (simp add: rga_ops_ref_exists x_pair)
       hence "r \<in> set (interp_rga xs)"
         using assms(2) interp_rga_ids rga_ops_rem_last by blast
       thus ?thesis by (simp add: split_list)
@@ -454,7 +169,7 @@ proof -
 qed
 
 lemma interp_rga_reorder:
-  assumes "valid_rga_ops (pre @ suf @ [(oid, ref)])"
+  assumes "rga_ops (pre @ suf @ [(oid, ref)])"
     and "\<And>i r. (i, Some r) \<in> set suf \<Longrightarrow> r \<noteq> oid"
     and "\<And>r. ref = Some r \<Longrightarrow> r \<notin> fst ` set suf"
   shows "interp_rga (pre @ (oid, ref) # suf) = interp_rga (pre @ suf @ [(oid, ref)])"
@@ -466,9 +181,13 @@ next
   have ref_not_x: "\<And>r. ref = Some r \<Longrightarrow> r \<noteq> fst x" using snoc.prems(3) by auto
   have IH: "interp_rga (pre @ (oid, ref) # xs) = interp_rga (pre @ xs @ [(oid, ref)])"
   proof -
-    have "valid_rga_ops (pre @ xs @ [(oid, ref)])"
-      using rga_ops_rem_penultimate ref_not_x
-      by (metis append.assoc prod.collapse snoc.prems(1))
+    have "rga_ops ((pre @ xs) @ [x] @ [(oid, ref)])"
+      using snoc.prems(1) by auto
+    moreover have "\<And>r. ref = Some r \<Longrightarrow> r \<noteq> fst x"
+      by (simp add: ref_not_x)
+    ultimately have "rga_ops ((pre @ xs) @ [(oid, ref)])"
+      using rga_ops_rem_penultimate
+      by (metis (no_types, lifting) Cons_eq_append_conv prod.collapse)
     thus ?thesis using snoc by force
   qed
   obtain xi xr where x_pair: "x = (xi, xr)" by force
@@ -493,8 +212,8 @@ qed
 
 lemma rga_spec_equal:
   assumes "permut xs ys"
-    and "valid_spec_ops xs"
-    and "valid_rga_ops ys"
+    and "spec_ops xs"
+    and "rga_ops ys"
   shows "interp_list xs = interp_rga ys"
 using assms proof(induction xs arbitrary: ys rule: rev_induct)
   case Nil
@@ -507,14 +226,32 @@ next
     using list_split_memb by force
   have IH: "interp_list xs = interp_rga (pre @ suf)"
   proof -
-    have "valid_rga_ops (pre @ suf)"
-      using rga_ops_rem_spec snoc by (metis ys_split spec_ops_last)
+    have "crdt_ops set_option (pre @ suf)"
+    proof -
+      have "crdt_ops set_option (pre @ [x] @ suf)"
+        using rga_ops_def snoc.prems(3) ys_split by blast
+      moreover have "opset (set (xs @ [x])) set_option"
+        by (metis insert_opset.axioms permut_def rga_ops_def snoc.prems(1) snoc.prems(3))
+      ultimately show "crdt_ops set_option (pre @ suf)"
+        using crdt_ops_rem_spec snoc.prems ys_split by blast
+    qed
+    moreover have "insert_opset (set (pre @ suf))"
+      using opset_sublist insert_opset.axioms insert_opset.intro rga_ops_def
+        snoc.prems(3) ys_split by blast
+    ultimately have "rga_ops (pre @ suf)"
+      using rga_ops_def by blast
     thus ?thesis
       using permut_rem_last spec_ops_rem_last ys_split snoc by metis
   qed
-  have valid_rga: "valid_rga_ops (pre @ suf @ [x])"
-    using rga_ops_reorder_spec snoc.prems ys_split
-    by (metis spec_ops_last)
+  have valid_rga: "rga_ops (pre @ suf @ [x])"
+  proof -
+    have "crdt_ops set_option (pre @ suf @ [x])"
+      using crdt_ops_reorder_spec snoc.prems ys_split
+      by (metis insert_opset.axioms permut_def rga_ops_def)
+    thus "rga_ops (pre @ suf @ [x])"
+      by (metis (no_types, lifting) append_Cons append_self_conv2 rga_ops_def
+          rotate1.simps(2) set_append set_rotate1 snoc.prems(3) ys_split)
+  qed
   have "interp_list (xs @ [x]) = interp_rga (pre @ suf @ [x])"
   proof -
     have "permut (xs @ [x]) (pre @ suf @ [x])"
@@ -527,10 +264,14 @@ next
   proof -
     obtain oid ref where x_pair: "x = (oid, ref)"
       by force
-    have "\<And>i r. (i, Some r) \<in> set suf \<Longrightarrow> r \<noteq> oid"
-      using rga_ops_independent_suf snoc.prems x_pair ys_split by blast
+    have "\<And>op2 r. op2 \<in> snd ` set suf \<Longrightarrow> r \<in> set_option op2 \<Longrightarrow> r \<noteq> oid"
+      using crdt_ops_independent_suf snoc.prems
+      by (metis insert_opset.axioms permut_def rga_ops_def x_pair ys_split)
+    hence "\<And>i r. (i, Some r) \<in> set suf \<Longrightarrow> r \<noteq> oid"
+      by fastforce 
     moreover have "\<And>r. ref = Some r \<Longrightarrow> r \<notin> fst ` set suf"
-      using rga_ops_no_future_ref snoc.prems(3) x_pair ys_split by blast
+      using crdt_ops_no_future_ref snoc.prems(3) x_pair ys_split
+      by (metis insert_opset.axioms option.set_intros rga_ops_def)
     ultimately show "interp_rga (pre @ suf @ [x]) = interp_rga (pre @ [x] @ suf)"
       using interp_rga_reorder valid_rga x_pair by force
   qed
@@ -539,42 +280,44 @@ next
 qed
 
 lemma spec_ops_exist:
-  assumes "valid_rga_ops xs"
-  shows "\<exists>ys. permut xs ys \<and> valid_spec_ops ys"
+  assumes "rga_ops xs"
+  shows "\<exists>ys. permut xs ys \<and> spec_ops ys"
 using assms proof(induction xs rule: List.rev_induct)
   case Nil
-  then show "\<exists>ys. permut [] ys \<and> valid_spec_ops ys"
-    by (simp add: permut_def valid_spec_ops.intros(1))
+  then show "\<exists>ys. permut [] ys \<and> spec_ops ys"
+    by (simp add: permut_def spec_ops_empty)
 next
   case (snoc x xs)
-  hence IH: "\<exists>ys. permut xs ys \<and> valid_spec_ops ys"
+  hence IH: "\<exists>ys. permut xs ys \<and> spec_ops ys"
     using rga_ops_rem_last by blast
   then obtain ys oid ref
-    where "permut xs ys" and "valid_spec_ops ys" and "x = (oid, ref)"
+    where "permut xs ys" and "spec_ops ys" and "x = (oid, ref)"
     by force
   moreover have "\<exists>pre suf. ys = pre@suf \<and>
                        (\<forall>i \<in> set (map fst pre). i < oid) \<and>
                        (\<forall>i \<in> set (map fst suf). oid < i)"
   proof -
-    have "oid \<notin> set (map fst ys)"
-      using permut_pair_fst rga_ops_unique_last calculation snoc.prems by blast
+    have "oid \<notin> set (map fst xs)"
+      using calculation(3) crdt_ops_unique_last rga_ops_def snoc.prems by fastforce
+    hence "oid \<notin> set (map fst ys)"
+      using calculation(1) permut_pair_fst by blast 
     thus ?thesis
-      using spec_ops_split \<open>valid_spec_ops ys\<close> by blast
+      using spec_ops_split \<open>spec_ops ys\<close> by blast
   qed
   from this obtain pre suf where "ys = pre @ suf" and
                        "\<forall>i \<in> set (map fst pre). i < oid" and
                        "\<forall>i \<in> set (map fst suf). oid < i" by force
   moreover have "permut (xs @ [(oid, ref)]) (pre @ [(oid, ref)] @ suf)"
-    using permut_append rga_ops_distinct calculation snoc.prems by fastforce
-  moreover have "valid_spec_ops (pre @ [(oid, ref)] @ suf)"
-    using rga_ops_ref_less_last spec_ops_add_any calculation snoc.prems by metis
-  ultimately show "\<exists>ys. permut (xs @ [x]) ys \<and> valid_spec_ops ys"
+    using permut_append crdt_ops_distinct calculation snoc.prems rga_ops_def by metis
+  moreover have "spec_ops (pre @ [(oid, ref)] @ suf)"
+    using spec_ops_add_any calculation by fastforce
+  ultimately show "\<exists>ys. permut (xs @ [x]) ys \<and> spec_ops ys"
     by blast
 qed
 
 theorem rga_meets_spec:
-  assumes "valid_rga_ops xs"
-  shows "\<exists>ys. permut ys xs \<and> valid_spec_ops ys \<and> interp_list ys = interp_rga xs"
+  assumes "rga_ops xs"
+  shows "\<exists>ys. permut ys xs \<and> spec_ops ys \<and> interp_list ys = interp_rga xs"
   using assms rga_spec_equal spec_ops_exist permut_commute by blast
 
 end
