isabelle/OpSet.thy
@@ -1,0 +1,428 @@
+theory OpSet
+  imports Main Permute Util
+begin
+
+definition spec_ops :: "('oid::{linorder} \<times> 'oper) list \<Rightarrow> bool" where
+  "spec_ops ops \<equiv> (sorted (map fst ops) \<and> distinct (map fst ops))"
+
+inductive crdt_ops :: "('oper \<Rightarrow> 'oid set) \<Rightarrow> ('oid::{linorder} \<times> 'oper) list \<Rightarrow> bool" where
+  "crdt_ops deps []" |
+  "\<lbrakk>crdt_ops deps xs;
+    oid \<notin> set (map fst xs);
+    \<forall>ref \<in> deps oper. ref \<in> set (map fst xs)\<rbrakk> \<Longrightarrow> crdt_ops deps (xs @ [(oid, oper)])"
+
+locale opset =
+  fixes opset :: "('oid::{linorder} \<times> 'oper) set"
+    and deps  :: "'oper \<Rightarrow> 'oid set"
+  assumes unique_oid: "(i1, op1) \<in> opset \<Longrightarrow> (i2, op2) \<in> opset \<Longrightarrow> op1 = op2"
+    and ref_older: "(oid, oper) \<in> opset \<Longrightarrow> ref \<in> deps oper \<Longrightarrow> ref < oid"
+    and finite_opset: "finite opset"
+
+lemma opset_subset:
+  assumes "opset Y deps"
+    and "X \<subseteq> Y"
+  shows "opset X deps"
+proof
+  fix i1 op1 i2 op2
+  assume "(i1, op1) \<in> X" and "(i2, op2) \<in> X"
+  thus "op1 = op2"
+    using assms by (meson opset.unique_oid set_mp)
+next
+  fix oid oper ref
+  assume "(oid, oper) \<in> X" and "ref \<in> deps oper"
+  thus "ref < oid"
+    using assms by (meson opset.ref_older set_rev_mp)
+next
+  show "finite X"
+    using assms opset.finite_opset finite_subset by blast
+qed
+
+lemma opset_insert:
+  assumes "opset (insert x ops) deps"
+  shows "opset ops deps"
+using assms opset_subset by blast
+
+lemma opset_sublist:
+  assumes "opset (set (xs @ ys @ zs)) deps"
+  shows "opset (set (xs @ zs)) deps"
+proof -
+  have "set (xs @ zs) \<subseteq> set (xs @ ys @ zs)"
+    by auto
+  thus "opset (set (xs @ zs)) deps"
+    using assms opset_subset by blast
+qed
+
+
+subsection\<open>Lemmata about the spec_ops predicate\<close>
+
+lemma spec_ops_empty:
+  shows "spec_ops []"
+by (simp add: spec_ops_def)
+
+lemma spec_ops_rem_last:
+  assumes "spec_ops (xs @ [x])"
+  shows "spec_ops xs"
+proof -
+  have "sorted (map fst (xs @ [x]))" and "distinct (map fst (xs @ [x]))"
+    using assms spec_ops_def by blast+
+  moreover from this have "sorted (map fst xs)" and "distinct xs"
+    by (auto simp add: sorted_append distinct_butlast distinct_map)
+  ultimately show "spec_ops xs"
+    using spec_ops_def by auto
+qed
+
+lemma spec_ops_id_inc:
+  assumes "spec_ops (xs @ [(oid, oper)])"
+    and "x \<in> set (map fst xs)"
+  shows "x < oid"
+proof -
+  have "sorted ((map fst xs) @ (map fst [(oid, oper)]))"
+    using assms(1) by (simp add: spec_ops_def)
+  hence "\<forall>i \<in> set (map fst xs). i \<le> oid"
+    by (simp add: sorted_append)
+  moreover have "\<forall>i \<in> set (map fst xs). i \<noteq> oid"
+    using assms(1) spec_ops_def by force
+  ultimately show "x < oid"
+    using assms(2) le_neq_trans by auto
+qed
+
+lemma spec_ops_add_any:
+  assumes "spec_ops (xs @ ys)"
+    and "\<forall>i \<in> set (map fst xs). i < oid"
+    and "\<forall>i \<in> set (map fst ys). oid < i"
+  shows "spec_ops (xs @ [(oid, oper)] @ ys)"
+using assms proof(induction ys rule: rev_induct)
+  case empty_ys: Nil
+  hence "sorted ((map fst xs) @ [oid])"
+    using assms(2) sorted_append spec_ops_def by fastforce
+  moreover have "distinct ((map fst xs) @ [oid])"
+    using empty_ys spec_ops_def by auto
+  ultimately show "spec_ops (xs @ [(oid, oper)] @ [])"
+    by (simp add: spec_ops_def)
+next
+  case (snoc y ys)
+  have IH: "spec_ops (xs @ [(oid, oper)] @ ys)"
+  proof -
+    from snoc have "spec_ops (xs @ ys)"
+      by (metis append_assoc spec_ops_rem_last)
+    thus "spec_ops (xs @ [(oid, oper)] @ ys)"
+      using assms(2) snoc by auto
+  qed
+  obtain yi yo where y_pair: "y = (yi, yo)"
+    by force
+  have oid_yi: "oid < yi"
+    by (simp add: snoc.prems(3) y_pair)
+  have yi_biggest: "\<forall>i \<in> set (map fst (xs @ [(oid, oper)] @ ys)). i < yi"
+  proof -
+    have "\<forall>i \<in> set (map fst xs). i < yi"
+      using oid_yi assms(2) less_trans by blast
+    moreover have "\<forall>i \<in> set (map fst ys). i < yi"
+      by (metis UnCI append_assoc map_append set_append snoc.prems(1) spec_ops_id_inc y_pair)
+    ultimately show ?thesis
+      using oid_yi by auto
+  qed
+  have "sorted (map fst (xs @ [(oid, oper)] @ ys @ [y]))"
+  proof -
+    from IH have "sorted (map fst (xs @ [(oid, oper)] @ ys))"
+      using spec_ops_def by blast
+    hence "sorted (map fst (xs @ [(oid, oper)] @ ys) @ [yi])"
+      using yi_biggest sorted_append
+      by (metis (no_types, lifting) append_Nil2 order_less_imp_le set_ConsD sorted_single)
+    thus "sorted (map fst (xs @ [(oid, oper)] @ ys @ [y]))"
+      by (simp add: y_pair)
+  qed
+  moreover have "distinct (map fst (xs @ [(oid, oper)] @ ys @ [y]))"
+  proof -
+    have "distinct (map fst (xs @ [(oid, oper)] @ ys) @ [yi])"
+      using IH yi_biggest spec_ops_def
+      by (metis distinct.simps(2) distinct1_rotate order_less_irrefl rotate1.simps(2))
+    thus "distinct (map fst (xs @ [(oid, oper)] @ ys @ [y]))"
+      by (simp add: y_pair)
+  qed
+  ultimately show "spec_ops (xs @ [(oid, oper)] @ ys @ [y])"
+    using spec_ops_def by blast
+qed
+
+lemma spec_ops_split:
+  assumes "spec_ops xs"
+    and "oid \<notin> set (map fst xs)"
+  shows "\<exists>pre suf. xs = pre @ suf \<and>
+            (\<forall>i \<in> set (map fst pre). i < oid) \<and>
+            (\<forall>i \<in> set (map fst suf). oid < i)"
+using assms proof(induction xs rule: rev_induct)
+  case Nil
+  then show ?case by force
+next
+  case (snoc x xs)
+  obtain xi xr where y_pair: "x = (xi, xr)"
+    by force
+  obtain pre suf where IH: "xs = pre @ suf \<and>
+               (\<forall>a\<in>set (map fst pre). a < oid) \<and>
+               (\<forall>a\<in>set (map fst suf). oid < a)"
+    by (metis UnCI map_append set_append snoc spec_ops_rem_last)
+  then show ?case
+  proof(cases "xi < oid")
+    case xi_less: True
+    have "\<forall>x \<in> set (map fst (pre @ suf)). x < xi"
+      using IH spec_ops_id_inc snoc.prems(1) y_pair by metis
+    hence "\<forall>x \<in> set suf. fst x < xi"
+      by simp
+    hence "\<forall>x \<in> set suf. fst x < oid"
+      using xi_less by auto
+    hence "suf = []"
+      using IH last_in_set by fastforce
+    hence "xs @ [x] = (pre @ [(xi, xr)]) @ [] \<and>
+              (\<forall>a\<in>set (map fst ((pre @ [(xi, xr)]))). a < oid) \<and>
+              (\<forall>a\<in>set (map fst []). oid < a)"
+      by (simp add: IH xi_less y_pair)
+    then show ?thesis by force
+  next
+    case False
+    hence "oid < xi" using snoc.prems(2) y_pair by auto
+    hence "xs @ [x] = pre @ (suf @ [(xi, xr)]) \<and>
+              (\<forall>i \<in> set (map fst pre). i < oid) \<and>
+              (\<forall>i \<in> set (map fst (suf @ [(xi, xr)])). oid < i)"
+      by (simp add: IH y_pair)
+    then show ?thesis by blast
+  qed
+qed
+
+lemma spec_ops_exists_base:
+  assumes "finite ops"
+    and "\<And>i1 i2 op1 op2. (i1, op1) \<in> ops \<Longrightarrow> (i2, op2) \<in> ops \<Longrightarrow> op1 = op2"
+  shows "\<exists>op_list. set op_list = ops \<and> spec_ops op_list"
+using assms proof(induct ops rule: Finite_Set.finite_induct_select)
+  case empty
+  then show "\<exists>op_list. set op_list = {} \<and> spec_ops op_list"
+    by (simp add: spec_ops_empty)
+next
+  case (select subset)
+  from this obtain op_list where "set op_list = subset" and "spec_ops op_list"
+    using assms(2) by blast
+  moreover obtain oid oper where select: "(oid, oper) \<in> ops - subset"
+    using select.hyps(1) by auto
+  moreover from this have "\<And>op2. (oid, op2) \<in> ops \<Longrightarrow> op2 = oper"
+    using assms(2) by auto
+  hence "oid \<notin> fst ` subset"
+    by (metis (no_types, lifting) DiffD2 select image_iff prod.collapse psubsetD select.hyps(1))
+  from this obtain pre suf
+    where "op_list = pre @ suf"
+      and "\<forall>i \<in> set (map fst pre). i < oid"
+      and "\<forall>i \<in> set (map fst suf). oid < i"
+    using spec_ops_split calculation by (metis (no_types, lifting) set_map)
+  moreover have "set (pre @ [(oid, oper)] @ suf) = insert (oid, oper) subset"
+    using calculation by auto
+  moreover have "spec_ops (pre @ [(oid, oper)] @ suf)"
+    using calculation spec_ops_add_any by fastforce
+  ultimately show ?case by blast
+qed
+
+lemma spec_ops_exists:
+  assumes "opset ops deps"
+  shows "\<exists>op_list. set op_list = ops \<and> spec_ops op_list"
+by (meson assms opset.finite_opset opset.unique_oid spec_ops_exists_base)
+
+
+subsection\<open>Lemmata about the crdt_ops predicate\<close>
+
+inductive_cases crdt_ops_last: "crdt_ops deps (xs @ [x])"
+
+lemma crdt_ops_intro:
+  assumes "\<And>r. r \<in> deps oper \<Longrightarrow> r \<in> fst ` set xs"
+    and "oid \<notin> fst ` set xs"
+    and "crdt_ops deps xs"
+  shows "crdt_ops deps (xs @ [(oid, oper)])"
+using assms crdt_ops.simps by force
+
+lemma crdt_ops_rem_last:
+  assumes "crdt_ops deps (xs @ [x])"
+  shows "crdt_ops deps xs"
+using assms crdt_ops.cases snoc_eq_iff_butlast by blast
+
+lemma crdt_ops_distinct:
+  assumes "crdt_ops deps xs"
+  shows "distinct xs"
+using assms by (induction xs, force+)
+
+lemma crdt_ops_distinct_fst:
+  assumes "crdt_ops deps xs"
+  shows "distinct (map fst xs)"
+using assms by (induction xs, auto)
+
+lemma crdt_ops_unique_last:
+  assumes "crdt_ops deps (xs @ [(oid, oper)])"
+  shows "oid \<notin> set (map fst xs)"
+using assms crdt_ops.cases by blast
+
+lemma crdt_ops_unique_mid:
+  assumes "crdt_ops deps (xs @ [(oid, oper)] @ ys)"
+  shows "oid \<notin> set (map fst xs) \<and> oid \<notin> set (map fst ys)"
+using assms proof(induction ys rule: rev_induct)  
+  case Nil
+  then show "oid \<notin> set (map fst xs) \<and> oid \<notin> set (map fst [])"
+    by (metis crdt_ops_unique_last Nil_is_map_conv append_Nil2 empty_iff empty_set)
+next
+  case (snoc y ys)
+  obtain yi yr where y_pair: "y = (yi, yr)"
+    by fastforce
+  have IH: "oid \<notin> set (map fst xs) \<and> oid \<notin> set (map fst ys)"
+    using crdt_ops_rem_last snoc by (metis append_assoc)
+  have "(xs @ (oid, oper) # ys) @ [(yi, yr)] = xs @ (oid, oper) # ys @ [(yi, yr)]"
+    by simp
+  hence "yi \<notin> set (map fst (xs @ (oid, oper) # ys))"
+    using crdt_ops_unique_last by (metis append_Cons append_self_conv2 snoc.prems y_pair)
+  thus "oid \<notin> set (map fst xs) \<and> oid \<notin> set (map fst (ys @ [y]))"
+    using IH y_pair by auto
+qed
+
+lemma crdt_ops_ref_exists:
+  assumes "crdt_ops deps (pre @ (oid, oper) # suf)"
+    and "ref \<in> deps oper"
+  shows "ref \<in> fst ` set pre"
+using assms proof(induction suf rule: List.rev_induct)
+  case Nil thus ?case
+    by (metis crdt_ops_last prod.sel(2))
+next
+  case (snoc x xs) thus ?case
+    using crdt_ops.cases by force
+qed
+
+lemma crdt_ops_no_future_ref:
+  assumes "crdt_ops deps (xs @ [(oid, oper)] @ ys)"
+    and "opset (set (xs @ [(oid, oper)] @ ys)) deps"
+  shows "\<And>ref. ref \<in> deps oper \<Longrightarrow> ref \<notin> fst ` set ys"
+proof -
+  from assms(1) have "\<And>ref. ref \<in> deps oper \<Longrightarrow> ref \<in> set (map fst xs)"
+    by (simp add: crdt_ops_ref_exists)
+  moreover have "distinct (map fst (xs @ [(oid, oper)] @ ys))"
+    using assms crdt_ops_distinct_fst by blast
+  ultimately have "\<And>ref. ref \<in> deps oper \<Longrightarrow> ref \<notin> set (map fst ([(oid, oper)] @ ys))"
+    using distinct_pair_list_memb by metis
+  thus "\<And>ref. ref \<in> deps oper \<Longrightarrow> ref \<notin> fst ` set ys"
+    by simp
+qed
+
+lemma crdt_ops_reorder:
+  assumes "crdt_ops deps (xs @ [(oid, oper)] @ ys)"
+    and "\<And>op2 r. op2 \<in> snd ` set ys \<Longrightarrow> r \<in> deps op2 \<Longrightarrow> r \<noteq> oid"
+  shows "crdt_ops deps (xs @ ys @ [(oid, oper)])"
+using assms proof(induction ys rule: rev_induct)
+  case Nil
+  then show "crdt_ops deps (xs @ [] @ [(oid, oper)])"
+    using crdt_ops_rem_last by auto
+next
+  case (snoc y ys)
+  then obtain yi yo where y_pair: "y = (yi, yo)"
+    by fastforce
+  have IH: "crdt_ops deps (xs @ ys @ [(oid, oper)])"
+  proof -
+    have "crdt_ops deps (xs @ [(oid, oper)] @ ys)"
+      by (metis snoc(2) append.assoc crdt_ops_rem_last)
+    thus "crdt_ops deps (xs @ ys @ [(oid, oper)])"
+      using snoc.IH snoc.prems(2) by auto
+  qed
+  have "crdt_ops deps (xs @ ys @ [y])"
+  proof -
+    have "yi \<notin> fst ` set (xs @ [(oid, oper)] @ ys)"
+      by (metis y_pair append_assoc crdt_ops_unique_last set_map snoc.prems(1))
+    hence "yi \<notin> fst ` set (xs @ ys)"
+      by auto
+    moreover have "\<And>r. r \<in> deps yo \<Longrightarrow> r \<in> fst ` set (xs @ ys)"
+    proof -
+      have "\<And>r. r \<in> deps yo \<Longrightarrow> r \<noteq> oid"
+        using snoc.prems(2) y_pair by fastforce
+      moreover have "\<And>r. r \<in> deps yo \<Longrightarrow> r \<in> fst ` set (xs @ [(oid, oper)] @ ys)"
+        by (metis y_pair append_assoc snoc.prems(1) crdt_ops_ref_exists)
+      ultimately show "\<And>r. r \<in> deps yo \<Longrightarrow> r \<in> fst ` set (xs @ ys)"
+        by simp
+    qed
+    moreover from IH have "crdt_ops deps (xs @ ys)"
+      using crdt_ops_rem_last by force
+    ultimately show "crdt_ops deps (xs @ ys @ [y])"
+      using y_pair crdt_ops_intro by (metis append.assoc)
+  qed
+  moreover have "oid \<notin> fst ` set (xs @ ys @ [y])"
+    using crdt_ops_unique_mid by (metis (no_types, lifting) UnE image_Un 
+      image_set set_append snoc.prems(1))
+  moreover have "\<And>r. r \<in> deps oper \<Longrightarrow> r \<in> fst ` set (xs @ ys @ [y])"
+    using crdt_ops_ref_exists
+    by (metis UnCI append_Cons image_Un set_append snoc.prems(1))
+  ultimately show "crdt_ops deps (xs @ (ys @ [y]) @ [(oid, oper)])"
+    using crdt_ops_intro by (metis append_assoc)
+qed
+
+lemma crdt_ops_rem_middle:
+  assumes "crdt_ops deps (xs @ [(oid, ref)] @ ys)"
+    and "\<And>op2 r. op2 \<in> snd ` set ys \<Longrightarrow> r \<in> deps op2 \<Longrightarrow> r \<noteq> oid"
+  shows "crdt_ops deps (xs @ ys)"
+using assms crdt_ops_rem_last crdt_ops_reorder append_assoc by metis
+
+lemma crdt_ops_independent_suf:
+  assumes "spec_ops (xs @ [(oid, oper)])"
+    and "crdt_ops deps (ys @ [(oid, oper)] @ zs)"
+    and "permut (xs @ [(oid, oper)]) (ys @ [(oid, oper)] @ zs)"
+    and "opset (set (xs @ [(oid, oper)])) deps"
+  shows "\<And>op2 r. op2 \<in> snd ` set zs \<Longrightarrow> r \<in> deps op2 \<Longrightarrow> r \<noteq> oid"
+proof -
+  have "\<And>op2 r. op2 \<in> snd ` set xs \<Longrightarrow> r \<in> deps op2 \<Longrightarrow> r < oid"
+  proof -
+    from assms(1) have "\<And>i. i \<in> fst ` set xs \<Longrightarrow> i < oid"
+      using spec_ops_id_inc by fastforce
+    moreover have "\<And>i2 op2 r. (i2, op2) \<in> set xs \<Longrightarrow> r \<in> deps op2 \<Longrightarrow> r < i2"
+      using opset.ref_older assms(4) by fastforce
+    ultimately show "\<And>op2 r. op2 \<in> snd ` set xs \<Longrightarrow> r \<in> deps op2 \<Longrightarrow> r < oid"
+      by fastforce
+  qed
+  moreover from assms(3) have "set zs \<subseteq> set xs"
+    by (metis permut_rem_last permut_subset(2))
+  ultimately show "\<And>op2 r. op2 \<in> snd ` set zs \<Longrightarrow> r \<in> deps op2 \<Longrightarrow> r \<noteq> oid"
+    by fastforce
+qed
+
+lemma crdt_ops_reorder_spec:
+  assumes "spec_ops (xs @ [x])"
+    and "crdt_ops deps (ys @ [x] @ zs)"
+    and "permut (xs @ [x]) (ys @ [x] @ zs)"
+    and "opset (set (xs @ [x])) deps"
+  shows "crdt_ops deps (ys @ zs @ [x])"
+using assms proof -
+  obtain oid oper where x_pair: "x = (oid, oper)" by force
+  hence "\<And>op2 r. op2 \<in> snd ` set zs \<Longrightarrow> r \<in> deps op2 \<Longrightarrow> r \<noteq> oid"
+    using assms crdt_ops_independent_suf by fastforce
+  thus "crdt_ops deps (ys @ zs @ [x])"
+    using assms(2) crdt_ops_reorder x_pair by metis
+qed
+
+lemma crdt_ops_rem_spec:
+  assumes "spec_ops (xs @ [x])"
+    and "crdt_ops deps (ys @ [x] @ zs)"
+    and "permut (xs @ [x]) (ys @ [x] @ zs)"
+    and "opset (set (xs @ [x])) deps"
+  shows "crdt_ops deps (ys @ zs)"
+using assms crdt_ops_rem_last crdt_ops_reorder_spec append_assoc by metis
+
+lemma crdt_ops_rem_penultimate:
+  assumes "crdt_ops deps (xs @ [(i1, r1)] @ [(i2, r2)])"
+    and "\<And>r. r \<in> deps r2 \<Longrightarrow> r \<noteq> i1"
+  shows "crdt_ops deps (xs @ [(i2, r2)])"
+proof -
+  have "crdt_ops deps (xs @ [(i1, r1)])"
+    using assms(1) crdt_ops_rem_last by force
+  hence "crdt_ops deps xs"
+    using crdt_ops_rem_last by force
+  moreover have "distinct (map fst (xs @ [(i1, r1)] @ [(i2, r2)]))"
+    using assms(1) crdt_ops_distinct_fst by blast
+  hence "i2 \<notin> set (map fst xs)"
+    by auto
+  moreover have "crdt_ops deps ((xs @ [(i1, r1)]) @ [(i2, r2)])"
+    using assms(1) by auto
+  hence "\<And>r. r \<in> deps r2 \<Longrightarrow> r \<in> fst ` set (xs @ [(i1, r1)])"
+    using crdt_ops_ref_exists by metis
+  hence "\<And>r. r \<in> deps r2 \<Longrightarrow> r \<in> set (map fst xs)"
+    using assms(2) by auto
+  ultimately show "crdt_ops deps (xs @ [(i2, r2)])"
+    by (simp add: crdt_ops_intro)
+qed
+
+
+end
